coq/JsPrettyRules.v
@@ -1111,8 +1111,8 @@ with red_expr : state -> execution_ctx -> ext_expr -> out -> Prop :=
       red_expr S C (expr_binary_op_add_string_1 y1) o ->
       red_expr S0 C (expr_binary_op_add_1 (ret S (v1,v2))) o
 
-  | red_expr_binary_op_add_string_1 : forall S0 S C s1 s2 s o,
-      s = string_concat s1 s2 ->
+  | red_expr_binary_op_add_string_1 : forall S0 S C s1 s2 s,
+      s = String.append s1 s2 ->
       red_expr S0 C (expr_binary_op_add_string_1 (ret S (value_prim s1, value_prim s2))) (out_ter S s)
 
   | red_expr_binary_op_add_1_number : forall S0 S C v1 v2 y1 o,
@@ -1136,7 +1136,7 @@ with red_expr : state -> execution_ctx -> ext_expr -> out -> Prop :=
 
   (** Binary op : shift operations (11.7) *)
 
-  | red_expr_shift_op : forall S C op b_unsigned F ext v1 v2 y1 o,
+  | red_expr_shift_op : forall b_unsigned S C op  F ext v1 v2 y1 o,
       shift_op op b_unsigned F ->
       ext = (if b_unsigned then spec_to_uint32 else spec_to_int32) ->
       red_spec S C (ext v1) y1 ->
@@ -1164,7 +1164,7 @@ with red_expr : state -> execution_ctx -> ext_expr -> out -> Prop :=
       red_expr S C (expr_inequality_op_2 b_swap b_neg y1) o ->
       red_expr S C (expr_inequality_op_1 b_swap b_neg v1 v2) o
 
-  | red_expr_inequality_op_2 : forall S0 S C (w1 w2 wa wb wr wr':prim) b (b_swap b_neg : bool),
+  | red_expr_inequality_op_2 : forall S0 S C (w1 w2 wa wb wr wr':prim) (b_swap b_neg : bool),
       ((wa,wb) = if b_swap then (w2,w1) else (w1,w2)) ->
       wr = inequality_test_primitive wa wb ->
       (* Note: wr may only be true or false or undef *)
@@ -3478,7 +3478,7 @@ with red_expr : state -> execution_ctx -> ext_expr -> out -> Prop :=
 
    (** Function: HasInstance  (returns bool)  (15.3.5.3) *)
 
-   | red_spec_object_has_instance_1_function_prim : forall S C l w o, (* Step 1 *)
+   | red_spec_object_has_instance_1_function_prim : forall S C l w, (* Step 1 *)
        red_expr S C (spec_object_has_instance_1 builtin_has_instance_function l (value_prim w)) (out_ter S false)
   
    | red_spec_object_has_instance_1_function_object : forall o1 S C l lv o, (* Step 2 *)
